---
title: "Untitled"
output: pdf_document
date: "2023-05-03"
---

## Proof Question

Consider the following missingness-graph

![](/Users/joshuayamamoto/Downloads/m_graph.png)

Here we have that:

-   $X$ and $Y$ are partially observed variables
-   $R_X$ is the missingness mechanism for $X$ and $R_Y$ is the missingness mechanism for $Y$
-   $X^*$ is a proxy variable for $X$ and $Y^*$ is a proxy for $Y$

Recall that for a partially observed variable $V$, the proxy variable $V^*$ is expressed as

- $V^* = (1- R_V)\cdot V + R_V\cdot m$


(a) Using the missigness-graph, show that the quantity $P(X,Y)$ is *recoverable*, i.e that it can be expressed in terms of fully observed terms.

(b) In words describe how $P(X, Y)$ can be estimated from the dataset using your final expression.




### Solution 

(a)

From the missingness-graph we can see that we have

- $X$ is independent of $R_X$ 
- $Y$ is conditionally independent of $R_X \ \cup \ R_Y$ given $X$

So we have that

$$
\begin{aligned}
P(X, Y) &= P(Y | X)P(X) \\
        &= P(Y | R_X, R_Y, X)P(X | R_X) 
\end{aligned}
$$

in particular

$$
\begin{aligned}
P(X, Y) &= P(Y | R_X = 0, R_Y = 0, X)P(X | R_X = 0)  \\
&= P(Y^* | X^*, R_X = 0, R_Y = 0 )P(X^* | R_X = 0)
\end{aligned}
$$

and all of these terms are observables.


(b)

We start by deleting all cases in which $X$ is missing in our dataset and estimate $P(X)$ from that. We then further remove all cases in which $Y$ is missing from that dataset where we removed cases where $X$ was missing and use this to estimate $P(Y | X)$.
